@prefix rdf: <http://www.w3.org/1999/02/22-rdf-syntax-ns#> .
@prefix owl: <http://www.w3.org/2002/07/owl#> .
@prefix dc: <http://purl.org/dc/elements/1.1/> .
@prefix xsd: <http://www.w3.org/2001/XMLSchema#> .
@prefix vann: <http://purl.org/vocab/vann/> .
@prefix foaf: <http://xmlns.com/foaf/0.1/> .
@prefix ssem: <http://purl.org/ssem/core/1.0.0/> .
@prefix rdfs: <http://www.w3.org/2000/01/rdf-schema#> .

<http://localhost:8080/neologism/ssem> a owl:Ontology;
    dc:title "SSEM Vocabulary";
    dc:modified "2013-09-17"^^xsd:date;
    vann:preferredNamespaceUri "http://purl.org/ssem/core/1.0.0/";
    vann:preferredNamespacePrefix "ssem";
    foaf:page <http://localhost:8080/neologism/ssem.html>;
    dc:creator <http://localhost:8080/neologism/ssem#robbinsd> .

<http://localhost:8080/neologism/ssem#robbinsd> a foaf:Person;
    foaf:name "David E. Robbins";
    foaf:homepage <http://about.me/robbinsd> .

<http://localhost:8080/neologism/ssem#Div.%20Informatics%2C%20Dept.%20Pathology%2C%20UAB> a foaf:Organization;
    foaf:member <http://localhost:8080/neologism/ssem#robbinsd>;
    foaf:name "Div. Informatics, Dept. Pathology, UAB";
    foaf:homepage <http://pathuab.infomedia.com/content.asp?id=490515> .

ssem:Constituent a rdfs:Class, owl:Class;
    rdfs:isDefinedBy <http://localhost:8080/neologism/ssem>;
    rdfs:label "Constituent";
    rdfs:comment "A constituent within a software ecosystem, such as a software system or an actor (e.g. user, developer, organization).";
    rdfs:subClassOf rdfs:Class .

ssem:Supplement a rdfs:Class, owl:Class;
    rdfs:isDefinedBy <http://localhost:8080/neologism/ssem>;
    rdfs:label "Supplemental Resource";
    rdfs:comment "A constituent within a software ecosystem, such as a software system or an actor (e.g. user, developer, organization).";
    rdfs:subClassOf rdfs:Class .

ssem:Relationship a rdfs:Class, owl:Class;
    rdfs:isDefinedBy <http://localhost:8080/neologism/ssem>;
    rdfs:label "Relationship";
    rdfs:comment "Class of all SSEM relationships.";
    rdfs:subClassOf rdf:Property .

ssem:supplementedBy a rdf:Property;
    rdfs:isDefinedBy <http://localhost:8080/neologism/ssem>;
    rdfs:label "is supplemented by";
    rdfs:comment "Links a Constituent or relationship to a Supplemental Resource.";
    rdfs:domain
        ssem:Constituent,
        ssem:Relationship;
    rdfs:range ssem:Supplement;
    rdfs:subPropertyOf ssem:relationship .

ssem:supplements a rdf:Property;
    rdfs:isDefinedBy <http://localhost:8080/neologism/ssem>;
    rdfs:label "supplements";
    rdfs:comment "Links a Supplemental Resource to the Constituent or relationship it supplements.";
    rdfs:domain ssem:Supplement;
    rdfs:range
        ssem:Relationship,
        ssem:Constituent;
    rdfs:subPropertyOf ssem:relationship .

ssem:relationship a rdf:Property;
    rdfs:isDefinedBy <http://localhost:8080/neologism/ssem>;
    rdfs:label "relationship";
    rdfs:comment "Super-property for all SSEM relationships between constituents, relationships, and supplements." .

ssem:interaction a rdf:Property;
    rdfs:isDefinedBy <http://localhost:8080/neologism/ssem>;
    rdfs:label "interaction";
    rdfs:comment "A relationship, or interaction, between two software ecosystem constituents.";
    rdfs:domain ssem:Constituent;
    rdfs:range ssem:Constituent;
    rdfs:subPropertyOf ssem:relationship .
